proofs up to lemma 18

theories/L/Complexity/Cook/GenNP_GenNPInter.v
@@ -22,6 +22,19 @@ Proof.
     eapply countIn. rewrite enum_ok. lia. 
 Qed. 
 
+
+Definition involution (X : Type) (f : X -> X) := forall (x : X), f (f x) = x. 
+
+Lemma map_involution (X : Type)(f : X -> X) : involution f -> involution (map f). 
+Proof. 
+  intros. intros l. rewrite map_map. setoid_rewrite H. now rewrite map_id. 
+Qed. 
+
+Lemma involution_invert_eqn (X : Type) (f : X -> X) : involution f -> forall a b, f a = f b -> a = b. 
+Proof. 
+  intros. enough (f (f a) = f(f b)) by (now repeat rewrite H). easy. 
+Qed. 
+
 Hint Resolve -> makeExhaustive_correct. 
 
 Section fixTM.
@@ -113,11 +126,11 @@ Section fixTM.
 
   (*flip the polarity of a symbol *)
   Definition polarityFlip p := match p with negative => positive | positive => negative | neutral => neutral end. 
-  Lemma polarityFlip_involutive p : polarityFlip(polarityFlip p) = p.
-  Proof. now destruct p. Qed. 
+  Lemma polarityFlip_involution : involution polarityFlip. 
+  Proof. intros p. now destruct p. Qed. 
   Definition polarityFlipSigma (x : polSigma) := match x with (p, σ) => (polarityFlip p, σ) end. 
-  Lemma polarityFlipSigma_involutive (x : polSigma) : polarityFlipSigma (polarityFlipSigma x) = x. 
-  Proof. destruct x, p; now cbn. Qed.
+  Lemma polarityFlipSigma_involution : involution polarityFlipSigma.
+  Proof. intros x. destruct x, p; now cbn. Qed.
 
   Definition polarityFlipTapeSigma' (x : tapeSigma') : tapeSigma' := match x with |_| => |_| | Some σ => Some (polarityFlipSigma σ) end. 
   Definition polarityFlipTapeSigma (x : tapeSigma) : tapeSigma := match x with inr a => inr (polarityFlipTapeSigma' a) | $ => $ end. 
@@ -127,21 +140,21 @@ Section fixTM.
   Notation "'#' x" := (polarityFlipTapeSigma' x) (at level 30). 
   Notation "'%' x" := (polarityFlipTapeSigma x) (at level 30). 
 
-  Lemma polarityFlipTapeSigma'_involutive (x: tapeSigma') : (##x) = x. 
-  Proof. destruct x; [ | now cbn]. cbn. now rewrite polarityFlipSigma_involutive. Qed. 
+  Lemma polarityFlipTapeSigma'_involution : involution polarityFlipTapeSigma'.
+  Proof. intros x. destruct x; [ | now cbn]. cbn. now rewrite polarityFlipSigma_involution. Qed. 
 
-  Lemma polarityFlipTapeSigma_involutive (x :tapeSigma) : (polarityFlipTapeSigma (polarityFlipTapeSigma x)) = x. 
+  Lemma polarityFlipTapeSigma_involution : involution polarityFlipTapeSigma.
   Proof.
-    destruct x; [ destruct d; now cbn | ]. cbn; now rewrite polarityFlipTapeSigma'_involutive.
+    intros x. destruct x; [ destruct d; now cbn | ]. cbn; now rewrite polarityFlipTapeSigma'_involution.
   Qed. 
-  Lemma polarityFlipGamma_involutive (x : Gamma) : (~~x) = x. 
+  Lemma polarityFlipGamma_involution : involution polarityFlipGamma. 
   Proof. 
-    destruct x; [now cbn | ]. cbn. now rewrite polarityFlipTapeSigma_involutive.  
+    intros x. destruct x; [now cbn | ]. cbn. now rewrite polarityFlipTapeSigma_involution.  
   Qed. 
 
   Lemma polarityFlipSigmaInv1 e p σ : polarityFlipSigma e = (p, σ) -> e = (polarityFlip p, σ). 
   Proof. 
-    unfold polarityFlipSigma. destruct e. intros. inv H. now rewrite polarityFlip_involutive.
+    unfold polarityFlipSigma. destruct e. intros. inv H. specialize (polarityFlip_involution p0). congruence. 
   Qed. 
 
   Lemma polarityFlipTapeSigmaInv1 e p σ : polarityFlipTapeSigma e = inr (Some (p, σ)) -> e = inr (Some (polarityFlip p, σ)). 
@@ -149,16 +162,22 @@ Section fixTM.
     unfold polarityFlipTapeSigma. destruct e.
     + destruct d. congruence. 
     + destruct e.  
-      - intros. inv H. destruct e. cbn in H1. inv H1. now rewrite polarityFlip_involutive.
+      - intros. inv H. destruct e. cbn in H1. inv H1. specialize (polarityFlip_involution p0) as ->. reflexivity.
       - cbn; congruence. 
   Qed. 
+  Lemma polarityFlipTapeSigma'Inv1 e p σ : polarityFlipTapeSigma' e = (Some (p, σ)) -> e = (Some (polarityFlip p, σ)). 
+  Proof.
+    unfold polarityFlipTapeSigma'. destruct e.  
+    - intros. inv H. destruct e. cbn in H1. inv H1. specialize (polarityFlip_involution p0) as -> ;reflexivity. 
+    - cbn; congruence. 
+  Qed.
 
   (*reverse a string + flip its polarities *)
   Definition polarityRev (x : list Gamma) : list Gamma := rev (map polarityFlipGamma x).
 
-  Lemma polarityRev_involutive (x : list Gamma) : polarityRev(polarityRev x) = x. 
+  Lemma polarityRev_involution : involution polarityRev.
   Proof. 
-    unfold polarityRev. rewrite map_rev, rev_involutive, map_map. setoid_rewrite polarityFlipGamma_involutive. 
+    intros x. unfold polarityRev. rewrite map_rev, rev_involutive, map_map. setoid_rewrite polarityFlipGamma_involution. 
     induction x; [eauto | cbn [map]; now rewrite IHx]. 
   Qed. 
 
@@ -197,6 +216,9 @@ Section fixTM.
 
   Hint Constructors rewHeadTape. 
 
+  (*help eauto to find the right constructor to apply *)
+  Hint Extern 4 (rewHeadTape _ ?H) => (match H with context[↓ ?e] => constructor 1 | context[↑ ?e] => constructor 2 | context [∘ ?e] => constructor 3 | _ => try (constructor 1; eauto); try (constructor 2; eauto) end); cbn.
+
   Lemma rewHeadTape_tail_invariant γ1 γ2 γ3 γ4 γ5 γ6 u v u' v' :
     rewHeadTape (γ1 :: γ2 :: γ3 :: u) (γ4 :: γ5 :: γ6 :: v) <-> rewHeadTape (γ1 :: γ2 :: γ3 :: u') (γ4 :: γ5 :: γ6 :: v').
   Proof. split; intros; inv H; eauto. Qed. 
@@ -229,13 +251,14 @@ Section fixTM.
   Proof. 
     intros. inv H. 
     - apply rewShiftRightTapeC. apply H1.
-    - apply rewShiftLeftTapeC. now repeat rewrite polarityFlipTapeSigma'_involutive.
+    - apply rewShiftLeftTapeC. now repeat rewrite polarityFlipTapeSigma'_involution.
     - apply identityWindow_revp in H1. now apply rewIdentityTapeC. 
   Qed. 
 
   Lemma rewHeadTape_revp γ1 γ2 γ3 γ4 γ5 γ6 : rewHeadTape [γ1; γ2; γ3] [γ4; γ5; γ6] <-> rewHeadTape [~γ3; ~γ2; ~γ1] [~γ6; ~γ5; ~γ4].
   Proof. 
-    split. apply rewHeadTape_revp'. intros H%rewHeadTape_revp'. now repeat rewrite polarityFlipGamma_involutive in H. 
+    split. apply rewHeadTape_revp'. intros H%rewHeadTape_revp'. specialize polarityFlipGamma_involution as H1. unfold involution in H1.
+    now repeat rewrite H1 in H.
   Qed.
 
   Lemma rewritesAt_rewHeadTape_add_at_end i a b u v : rewritesAt rewHeadTape i a b -> rewritesAt rewHeadTape i (a ++ u) (b ++ v).  
@@ -369,21 +392,52 @@ Section fixTM.
     + unfold withPolaritySigma in H3; congruence. 
   Qed. 
 
+  Lemma tape_repr_inv6 w p u us h : us :: u ≃t(p, w) h -> exists h' n, h = (inr (inr (Some (p, us)))):: h' ++ E (n + wo) /\ w = n + S (|h'|) /\ |h'| = |u| /\ u ≃t(p, w -1) h' ++ E (n + wo). 
+  Proof.
+    intros.
+    destruct h. { destruct H. cbn in H; lia. }
+    destruct H as (H1 & H2 & H3). 
+    cbn [mapPolarity length map] in H3. exists (mapPolarity p u), (w - S (|u|)). 
+    repeat split. 
+    - cbn in H2, H1. replace (w - S (|u|) + wo) with (w + wo - S (|u|)) by lia. apply H3. 
+    - unfold mapPolarity. rewrite map_length. cbn in H2. lia. 
+    - unfold mapPolarity. now rewrite map_length. 
+    - unfold mapPolarity. rewrite app_length, map_length. cbn in H1, H2. rewrite E_length. lia. 
+    - cbn in H2; lia. 
+    - cbn in H2. now replace (w - S (|u|) + wo) with (w - 1 + wo - (|u|)) by lia.
+  Qed.
+
+  Lemma tape_repr_inv7 w p u us n : us :: u ≃t(p, w) E n -> False. 
+  Proof. intros (H1 & H2 & H3). destruct n; cbn in H3; unfold withPolaritySigma in H3; congruence. Qed.
+
+  Lemma tape_repr_inv8 u us p w e rs : us :: u ≃t(p, w) inr(inr e) :: rs -> e = Some (p, us). 
+  Proof. intros (H1 & H2 & H3). cbn in H3. unfold withPolaritySigma in H3. congruence. Qed. 
+
+
   Ltac discr_tape := match goal with
                      | [ H : ?u ≃t(?p, ?w) (inl ?e) :: ?a |- _] => now apply tape_repr_inv in H
                      | [ H : [] ≃t(?p, ?w) (inr (inr (Some ?e))) :: ?a |- _] => now apply tape_repr_inv2 in H
                      | [ H : ?u :: ?us ≃t(?p, ?w) inr (inr |_|):: ?a |- _] => now apply tape_repr_inv3 in H
                      | [ H : ?u :: ?us ≃t(?p, ?w) inr $ :: ?a |- _] => now apply tape_repr_inv4 in H
                      | [H : _ ≃t(?p, ?w) inr $ :: ?e :: ?a |- _] => now apply tape_repr_inv5 in H
+                     | [H : ?u :: ?us ≃t(?p, 0) _ |- _] => destruct H; cbn in *; lia
+                     | [H : ?u :: ?us ≃t(?p, ?w) [] |- _] => let H1 := fresh in apply tape_repr_inv6 in H as (? & ? & (H1 & _ & _& _)); congruence
+                                                                                                                                        |[H : ?u :: ?us ≃t(?p, ?w) E ?n |- _] => now apply tape_repr_inv7 in H
                       end. 
+
 
   Ltac destruct_tape := repeat match goal with
                         | [H : _ ≃t(?p, ?w) ?x :: ?h |- _] => is_var x; destruct x; try discr_tape
                         | [H : _ ≃t(?p, ?w) (inr ?e) :: ?h |- _] => is_var e; destruct e; try discr_tape
                         | [H : ?u ≃t(?p, ?w) inr _ :: ?h |- _] => is_var u; destruct u; try discr_tape
                         | [H : delim |- _] => destruct H; try discr_tape
+                        | [H : [] ≃t(?p, ?w) (inr (inr ?e)) :: ?h |- _] => is_var e; destruct e; try discr_tape
+                        | [H : ?u :: ?us ≃t(?p, ?w) ?h |- _] => is_var h; destruct h; try discr_tape
+                        | [H: ?u :: ?us ≃t(?p, ?w) ?h' ++ ?h'' |- _] => is_var h'; destruct h'; try discr_tape
+                        | [H : ?u :: ?us ≃t(?p, ?w) inr(inr ?e) :: _ |- _] => is_var e; specialize (tape_repr_inv8 H) as ->  
                           end. 
 
+  Ltac cbn_friendly := cbn [polarityFlipGamma polarityFlipSigma polarityFlipTapeSigma polarityFlipTapeSigma' polarityFlip ].
   Ltac rewHeadTape_inv := repeat match goal with 
                                    | [H : rewHeadTape  ?a _ |- _] => is_var a; destruct a; try (inv H; fail)
                                    | [H : rewHeadTape  (_ :: ?a) _ |- _] => is_var a; destruct a; try (inv H; fail)
@@ -391,7 +445,15 @@ Section fixTM.
                                    | [H : rewHeadTape  _ ?a |- _ ] => is_var a; destruct a; try (inv H; fail)
                                    | [H : rewHeadTape  _ (_ :: ?a) |-_ ] => is_var a; destruct a; try (inv H; fail)
                                    | [H : rewHeadTape  _ (_ :: _ :: ?a) |- _] => is_var a; destruct a; try (inv H; fail)
-                               end.
+                                                             
+                               end; cbn_friendly.
+
+  Lemma polarityFlip_push_in (σ : tapeSigma') : inr (inr (polarityFlipTapeSigma' σ)) = polarityFlipGamma (inr (inr σ)). 
+  Proof. now cbn. Qed. 
+
+  Create HintDb tape discriminated.
+  Hint Rewrite polarityFlipSigma_involution : tape. 
+  Hint Rewrite polarityFlip_involution : tape. 
 
   Ltac rewHeadTape_inv2 := repeat match goal with
                                   | [H : rewHeadTape _ _ |- _] => inv H
@@ -399,15 +461,18 @@ Section fixTM.
                                   | [H : identityWindow _ _ _ _ _ _ |- _] => inv H
                                   | [H : |_| = # ?σ |- _] => is_var σ; destruct σ; cbn in H; try congruence
                                   | [H : # ?σ = |_| |- _] => is_var σ; destruct σ; cbn in H; try congruence
-                                  | [H : Some (_, _) = # ?e |- _] => symmetry in H; apply polarityFlipTapeSigmaInv1 in H; rewrite H in *; clear H
-                                  | [H : # ?e = Some (_, _) |- _] => apply polarityFlipTapeSigmaInv1 in H; rewrite H in *; clear H
+                                  | [H : Some (_, _) = % ?e |- _] => symmetry in H; apply polarityFlipTapeSigmaInv1 in H; rewrite H in *; clear H
+                                  | [H : % ?e = Some (_, _) |- _] => apply polarityFlipTapeSigmaInv1 in H; rewrite H in *; clear H
+                                  | [H : Some (_, _) = # ?e |- _] => symmetry in H; apply polarityFlipTapeSigma'Inv1 in H; rewrite H in *; clear H
+                                  | [H : # ?e = Some (_, _) |- _] => apply polarityFlipTapeSigma'Inv1 in H; rewrite H in *; clear H
                                   | [H : |_| = |_| |- _] => clear H
-                           end. 
+                                  | [ |- context [inr (inr (# ?e))]] => rewrite polarityFlip_push_in
+                           end; cbn_friendly. 
  
-  Lemma tape_rewrite_symm1 u h p h' : u ≃t(p) h -> valid rewHeadTape h h' -> valid rewHeadTape (polarityRev h) (polarityRev h'). 
+  (*Lemma 15 *)
+  Lemma tape_rewrite_symm1 u h p n h' : u ≃t(p, n) h -> valid rewHeadTape h h' -> valid rewHeadTape (polarityRev h) (polarityRev h'). 
   Proof.
-    intros.
-    unfold reprTape in H. revert u H. generalize z'. 
+    intros. revert n u H. 
     induction H0; intros. 
     - cbn; constructor. 
     - apply reprTape_length in H1. cbn [length] in H1; unfold wo in H1. lia.  
@@ -453,14 +518,14 @@ Section fixTM.
   Qed. 
 
   Lemma polarityRev_eqn_move a b : a = polarityRev b -> b = polarityRev a. 
-  Proof. intros ->; symmetry; now apply polarityRev_involutive. Qed. 
+  Proof. intros ->; symmetry; now apply polarityRev_involution. Qed. 
 
-  Lemma tape_rewrite_symm2 u h p h' : u ≃t(p) h -> valid rewHeadTape (polarityRev h) (polarityRev h') -> valid rewHeadTape h h'.
+  Lemma tape_rewrite_symm2 u h p n h' : u ≃t(p, n) h -> valid rewHeadTape (polarityRev h) (polarityRev h') -> valid rewHeadTape h h'.
   Proof.
     (*the proof is structurally very similar to the proof for tape_rewrite_symm1, *)
     (*but not a direct consequence since the tape h is not reversed; *)
     (*the reversion poses an additional challenge for tape inversion*)
-    intros. unfold reprTape in H. revert u H. generalize z'. 
+    intros. revert n u H.  
     remember (polarityRev h). remember (polarityRev h').
     apply polarityRev_eqn_move in Heql0 as ->. apply polarityRev_eqn_move in Heql1 as ->. 
     induction H0; intros.
@@ -509,15 +574,194 @@ Section fixTM.
 
   Admitted. 
 
-  Lemma tape_rewrite_symm3 u h p h' : u ≃t(p) h -> valid rewHeadTape h h' -> valid rewHeadTape (map polarityFlipGamma h) h'. 
+  Lemma tape_rewrite_symm3 h h' :valid rewHeadTape h h' -> valid rewHeadTape (map polarityFlipGamma h) h'. 
   Proof. 
-    intros. induction H0. 
+    intros. unfold reprTape in H. induction H; intros. 
     - cbn; constructor. 
-    - 
-  Admitted. 
+    - cbn [map polarityFlipGamma]. constructor. 2: now rewrite map_length. apply IHvalid.  
+    - cbn [map polarityFlipGamma]. rewHeadTape_inv. constructor 3. 
+      + (* want to apply the IH *)
+        apply IHvalid. 
+      + cbn [map polarityFlipGamma]. apply rewHeadTape_tail_invariant with (u' := a) (v' := b). 
+        rewHeadTape_inv2; try rewrite polarityFlip_involutive; eauto.
+  Qed. 
 
-  
+  Lemma valid_base sig (p : rewritesHeadAbstract sig) (a b c d e f : sig) : valid p [a; b ; c] [d; e; f] <-> p [a; b; c] [d; e; f]. 
+  Proof. 
+    split.
+    - intros; inv H. cbn in H5; lia. apply H5.  
+    - constructor 3. 2: apply H. repeat constructor.
+  Qed. 
 
+  (*Lemma 16 *)
+  Lemma E_rewrite_blank n : valid rewHeadTape (E (S (S n))) (E (S (S n))). 
+  Proof. 
+    intros. induction n. 
+    + apply valid_base. eauto. 
+    + constructor 3. 
+      - cbn [E] in IHn. now apply IHn. 
+      - eauto. 
+  Qed. 
+
+  Ltac inv_valid := match goal with
+                      | [ H : valid _ _ _ |- _] => inv H
+                    end;
+                    try match goal with
+                    | [ H : | _ | < 2 |- _] => now cbn in H
+                    end.
+
+  Lemma E_rewrite_blank_unique' n : n >= 1 -> forall s, valid rewHeadTape (E (S n)) (inr (inr |_|) :: s) -> s = E n. 
+  Proof. 
+    intros H. induction n; intros; [lia | ]. 
+    destruct n; cbn [E] in *. 
+    + inv_valid. rewHeadTape_inv2. 
+      apply valid_length_inv in H4. inv H4. now (destruct v; cbn in H1).
+    + inv_valid. rewHeadTape_inv2. 
+      * eapply IHn in H4. congruence. lia. 
+      * f_equal. now eapply IHn. 
+  Qed. 
+  Corollary E_rewrite_blank_unique n : forall s, valid rewHeadTape (E (S (S n))) (inr (inr |_|) :: s) -> s = E (S n).  
+  Proof. intros; now apply E_rewrite_blank_unique'. Qed.
+
+  (*Lemma 17 *)
+  Lemma E_rewrite_sym σ n: valid rewHeadTape (E (S (S (S n)))) (inr (inr (Some (↑σ))) :: E (S (S n))). 
+  Proof. 
+    intros. cbn [E] in *.
+    constructor 3. 
+    - apply E_rewrite_blank. 
+    - eauto. 
+  Qed. 
+
+  Lemma E_rewrite_sym_unique σ n : forall (s : string Gamma), valid rewHeadTape (E (S (S (S n)))) (inr (inr (Some (↑ σ))) :: s) -> s = E (S (S n)). 
+  Proof. 
+    intros. inv_valid. rewHeadTape_inv2. cbn [E]. f_equal. apply E_rewrite_blank_unique in H3. auto. 
+  Qed. 
+
+  Lemma E_polarityFlip n : map polarityFlipGamma (E n) = E n. 
+  Proof. induction n; cbn; now f_equal. Qed. 
+
+  Lemma E_rewrite_sym_rev σ n : valid rewHeadTape (rev (E (S (S (S n))))) (rev (inr (inr (Some (↓ σ))) :: E (S (S n)))). 
+  Proof. 
+    (*follows using tape_rewrite_symm1, tape_rewrite_symm3 and E_rewrite_sym *)
+    specialize (E_rewrite_sym σ n) as H1. 
+    eapply tape_rewrite_symm1 in H1. 2: replace ((S (S (S n)))) with ((S n + wo)) by (unfold wo; lia).
+    - eapply tape_rewrite_symm3 in H1.
+      unfold polarityRev in H1. rewrite map_rev, map_map in H1. setoid_rewrite polarityFlipGamma_involution in H1. rewrite map_id in H1. 
+      cbn [map polarityFlipGamma polarityFlipTapeSigma polarityFlipTapeSigma' polarityFlipSigma polarityFlip] in H1. 
+      now rewrite E_polarityFlip in H1. 
+    - eapply niltape_repr with (p := positive). 
+  Qed. 
+
+  Lemma E_rewrite_sym_rev_unique σ n : forall s, valid rewHeadTape (rev (E (S (S (S n))))) (rev (inr (inr (Some (↓ σ))) :: s)) -> s = E (S (S n)). 
+  Proof. 
+    intros.
+    assert (valid rewHeadTape (polarityRev (E (S (S (S n))))) (polarityRev (inr (inr (Some (↑ σ))) :: map polarityFlipGamma s))). 
+    {
+      unfold polarityRev. rewrite E_polarityFlip. cbn [map]. cbn_friendly. rewrite map_involution. 2: apply polarityFlipGamma_involution.
+      apply H. 
+    }
+    eapply tape_rewrite_symm2 in H0.
+    - apply E_rewrite_sym_unique in H0. 
+      enough (map polarityFlipGamma (E (S (S n))) = E (S (S n))).
+      { rewrite <- H1 in H0. apply involution_invert_eqn in H0. assumption. apply map_involution, polarityFlipGamma_involution. }
+      apply E_polarityFlip. 
+   - replace ((S (S (S n)))) with (S n + wo) by (unfold wo; lia). eapply niltape_repr with (p := positive). 
+  Qed. 
+
+  (*Lemma 18 *)
+  Definition setPolarityGamma p γ := match γ with inr (inr (Some (_, σ))) => inr (inr (Some (p, σ))) | _ => γ end. 
+  Notation "p '@' γ" := (setPolarityGamma p γ) (at level 60).
+
+  Lemma apply_fun_eqn {X Y : Type} (f : X -> Y) (a b : X) : a = b -> f a = f b. 
+  Proof. now intros ->. Qed. 
+
+
+
+
+  Lemma tape_repr_add_right rs σ h p w: rs ≃t(p, w) h -> length rs < w -> exists h', valid rewHeadTape h (inr (inr (Some (↑ σ))) :: h')  /\ σ :: rs ≃t(positive, w)  (inr (inr (Some (↑ σ))) :: h'). 
+  Proof. 
+    intros. revert w h σ H H0. 
+    induction rs.
+    - intros. apply niltape_repr in H as ->. exists (E (w + wo - 1)). split. 
+      + cbn in H0. destruct w; [lia | ]. unfold wo. replace (S w + 2) with (S (S (S w))) by lia. cbn [Nat.sub]. apply E_rewrite_sym.
+      + repeat split. 
+        * cbn. rewrite E_length. lia. 
+        * now cbn. 
+    - intros. apply tape_repr_inv6 in H as (h' & n & -> & -> & H2 & H3).
+      replace (n + S (|h'|) - 1) with (n + |h'|) in H3 by lia.
+      destruct rs; [ | destruct rs].
+      + (*at the end of the used tape region *)
+        destruct h'; [clear H2 | now cbn in H2]. clear H3. 
+        destruct n; [cbn in H0; cbn in H0; lia | ]. exists (inr (inr (Some (↑a))):: E (n + wo)). split.
+        * cbn [app]. rewrite Nat.add_comm. setoid_rewrite Nat.add_comm at 2. unfold wo. cbn [Nat.add Nat.sub]. constructor 3. 
+          -- apply E_rewrite_sym. 
+          -- cbn [E]. apply rewHeadTape_tail_invariant with (u' := []) (v' := []). eauto. 
+        * repeat split. 
+          -- cbn. rewrite E_length. cbn in H0. lia. 
+          -- cbn; cbn in H0; lia. 
+          -- cbn. unfold withPolaritySigma. now replace (n + 1 + wo - 1) with (n + wo) by lia. 
+      + (* rs has length 1*)
+        destruct_tape. cbn [app] in H3; discr_tape. 
+        destruct h'; [ | now cbn in H2]. clear H2. 
+        cbn [app] in H3. destruct_tape. cbn [length] in *. 
+        destruct n; [lia | ]. clear H0. 
+        exists (inr(inr (Some (↑a))) :: inr (inr (Some (↑e))) :: E (n + wo)). 
+        cbn [app]; split. 
+        * constructor 3. 
+          -- unfold wo. replace (S n + 2) with (S(S (S n))) by lia. rewrite Nat.add_comm. constructor 3. 
+             ++ apply E_rewrite_sym. 
+             ++ cbn [E]. apply rewHeadTape_tail_invariant with (u' := [] ) (v' := []); eauto. 
+          -- cbn[E]. apply rewHeadTape_tail_invariant with (u' := []) (v' := []). eauto. 
+        * repeat split.
+          -- cbn. rewrite E_length. lia. 
+          -- cbn; lia. 
+          -- cbn[mapPolarity map length app]. now replace (S n + 2 + wo - 3) with (n + wo) by lia. 
+     + (*rs has at least two elements. this is the interesting case as it needs the IH *) 
+       destruct_tape. cbn [app] in H3; discr_tape. cbn [length app] in H3. rewrite Nat.add_succ_r in H3. 
+       apply tape_repr_step in H3 as H4. destruct_tape. cbn [app] in H4; discr_tape. 
+       cbn [app length] in *. destruct_tape. 
+
+       (*we use the IH with h := inr (...e) :: inr (...e0) :: h' ++ E(n + wo); w := S (S (n + |h'|)); σ := a *)
+       rewrite Nat.add_succ_r in H3. specialize (IHrs _ _ a H3). 
+       edestruct (IHrs) as (h'' & F1 & F2). lia. 
+       exists (inr (inr (Some (↑a))) :: h'').
+       (*we need to know one more symbol at the head of h'' for the proof *)
+       apply tape_repr_step in F2 as F3. destruct_tape. 
+       split.
+       * constructor 3.  
+         -- apply F1. 
+         -- apply rewHeadTape_tail_invariant with (u' := []) (v' := []); eauto. 
+       * repeat split.
+         -- cbn. destruct F2 as (F2 & _ & _). cbn in F2. lia.  
+         -- cbn. destruct F2 as (_ & F2 & _). cbn in F2. lia. 
+         -- destruct F2 as (_ & _ & ->). cbn[app length Nat.add Nat.sub].
+            replace (n + S (S (S (|h'|))) + wo - (S (S (S (S(|rs|)))))) with (n + (|h'|) + wo - S(|rs|)) by lia.
+            easy. 
+  Qed. 
+
+  Lemma tape_repr_polarityFlip ls p w h : ls ≃t(p, w) h -> ls ≃t(polarityFlip p, w) map polarityFlipGamma h. 
+  Proof. 
+    intros (H1 & H2 & H3). repeat split. 
+    - now rewrite map_length. 
+    - apply H2.
+    - rewrite H3. unfold mapPolarity, polarityFlipGamma. rewrite map_app. rewrite map_map. 
+      rewrite E_polarityFlip. easy. 
+  Qed. 
+
+  Corollary tape_repr_add_left ls σ h p w: ls ≃t(p, w) h -> length ls < w -> exists h', valid rewHeadTape (rev h) (rev (inr (inr (Some (↓ σ))) :: h'))  /\ σ :: ls ≃t(negative, w)  (inr (inr (Some (↓ σ))) :: h').
+  Proof. 
+    intros. specialize (@tape_repr_add_right ls σ h p w H H0) as (h' & H1 & H2). 
+    eapply tape_rewrite_symm1 with (u:= ls) (p := p) (n:=w)in H1. 2: apply H. 
+    apply tape_rewrite_symm3 in H1.
+    exists (map polarityFlipGamma h'). split. 
+    - cbn [rev].
+      cbn[polarityRev map rev polarityFlipGamma polarityFlipTapeSigma polarityFlipTapeSigma' polarityFlipSigma polarityFlip] in H1.
+      unfold polarityRev in H1. rewrite map_rev in H1. rewrite map_involution in H1. 2: apply polarityFlipGamma_involution. 
+      apply H1. 
+   - apply tape_repr_polarityFlip in H2. cbn in H2. easy. 
+  Qed. 
+
+  (**TODO: uniqueness*)
 
 End fixTM. 
 
